src/LibEnv.v
@@ -1,3 +1,5 @@
+(* -- TODO
+
 (**************************************************************************
 * TLC: A library for Coq                                                  *
 * Environments for metatheory                                             *
@@ -1253,3 +1255,4 @@ Ltac binds_cases_base H :=
 
 
 
+*)
