src/LibFun.v
@@ -1,3 +1,5 @@
+(* -- TODO DEPRECATED?
+
 (**************************************************************************
 * TLC: A library for Coq                                                  *
 * Functions                                                               *
@@ -245,3 +247,6 @@ Proof using. introv I. induction n; introv Hx; autos*. Qed.
 
 (* TODO: rename applyn to iter *)
 (* TODO: migrate iteration of functionals from LibFix to here *)
+
+
+*)
